typeclass_typing: update typing and class constraint elaboration rules

typeclass/typing/typeclass_typingScript.sml
@@ -3,12 +3,12 @@ open pairTheory arithmeticTheory integerTheory stringTheory optionTheory
      listTheory alistTheory;
 open typeclass_typesTheory typeclass_tcexpTheory
 typeclass_kindCheckTheory pure_configTheory;
-open typeclass_env_mapTheory;
 open monadsyntax;
+
+(* open typeclass_env_mapTheory; *)
 
 val _ = monadsyntax.enable_monadsyntax();
 val _ = monadsyntax.enable_monad "option";
-
 
 val _ = new_theory "typeclass_typing";
 
@@ -90,18 +90,14 @@ Definition type_ok_def:
   type_ok typedefs ks t = kind_ok typedefs ks kindType t
 End
 
-Definition pred_type_well_scoped_def: 
+Definition pred_type_well_scoped_def:
   pred_type_well_scoped (Pred ps t) =
   (∀cl v. MEM (cl,v) ps ⇒
     collect_type_vars v ⊆ collect_type_vars t)
 End
 
 Definition pred_type_kind_ok_def:
-  pred_type_kind_ok (cl_map:class_map) (typedefs: typedefs) ks pt ⇔
-    let cldb s = do
-      clinfo <- FLOOKUP cl_map s;
-      clinfo.kind
-    od in
+  pred_type_kind_ok cldb (typedefs: typedefs) ks pt ⇔
     pred_kind_wf cldb (typedefs_to_cdb typedefs) (LLOOKUP ks) pt
 End
 
@@ -124,6 +120,21 @@ Theorem type_ok_IMP_freetyvars_ok:
 Proof
   metis_tac[kind_ok_IMP_freetyvars_ok,type_ok_def]
 QED
+
+Type pred_type_scheme[pp] = ``:Kind list # PredType``;
+Type type_scheme[pp] = ``:Kind list # type``;
+
+Overload subst_db_scheme =
+  ``λn ts (vars,scheme).
+      (vars, subst_db (n + vars) (MAP (shift_db 0 vars) ts) scheme)``;
+Overload shift_db_scheme =
+  ``λskip shift (vars,scheme).
+      (vars, shift_db (skip + vars) shift scheme)``;
+Overload tshift_scheme = ``λn (vars,scheme). (vars, shift_db vars n scheme)``;
+Overload tshift_scheme_pred = ``λn (vars,scheme). (vars, shift_db_pred
+(LENGTH vars) n scheme)``;
+Overload tshift_env = ``λn. MAP (λ(x,scheme). (x, tshift_scheme n scheme))``;
+Overload tshift_env_pred = ``λn. MAP (λ(x,scheme). (x, tshift_scheme_pred n scheme))``;
 
 Overload type_scheme_ok =
   ``λtdefs ks (varks,scheme). type_ok tdefs (ks ++ varks) scheme``
@@ -237,20 +248,18 @@ Inductive type_atom_op:
   (s ≠ "" ⇒ type_atom_op (Message s) [String] Message)
 End
 
-(* TODO: notes: probably don't need it as we have kind checking
 (* Typing judgments for type constructors *)
 Definition type_cons_def:
-  type_cons (typedefs : typedefs) (cname,carg_tys) (tyid,tyargs) ⇔
+  type_cons (typedefs : typedefs) db (cname,carg_tys) (tyid,tyargs) ⇔
     ∃argks constructors schemes.
       (* There is some type definition: *)
         oEL tyid typedefs = SOME (argks, constructors) ∧
       (* Which declares the constructor: *)
         ALOOKUP constructors cname = SOME schemes ∧
       (* And we can specialise it appropriately: *)
-        LIST_REL (λk tyarg. kind_ok typedefs ) argks tyargs ∧
+        LIST_REL (kind_ok typedefs db) argks tyargs ∧
         MAP (tsubst tyargs) schemes = carg_tys
 End
-*)
 
 (* Typing judgments for exceptions *)
 Definition type_exception_def:
@@ -264,93 +273,352 @@ Definition get_PrimTys_def:
   get_PrimTys _ = NONE
 End
 
-(*
-  The main typing relation.
-  type_tcexp :
-      exndef # typedefs           -- type definitions for exceptions and datatypes
-   -> num                         -- number of deBruijn indices in scope
-   -> type list                   -- store typing
-   -> (string # type_scheme) list -- term variables associated to type schemes
-   -> tcexp -> type                -- expression and its type
-*)
-
-Definition user_annot_ok_def:
-  (user_annot_ok NONE pt ⇔ T) ∧
-  (user_annot_ok (SOME ut) pt ⇔ ut = pt)
-End
 
 Datatype:
-  inst_type = Instance [(mlstring # type)] (mlstring # type)
+  entailment = Entail ((mlstring # type) list) (mlstring # type)
 End
 
+Definition specialises_inst_def:
+  specialises_inst (Entail ps p) (Entail qs q) ⇔
+    ∃subs.
+      LIST_REL (λ(c,t) (c',t'). c = c' ∧ tsubst subs t = t') (p::ps) (q::qs)
+    (*
+    * ∃subs. FST p = FST q ∧  
+      tsubst subs (SND p) = (SND q) ∧
+      (∀c v. MEM (c,v) ps ⇒
+        MEM (c,tsubst subs v) qs) *)
+End
+
+(* if s is a super class of c then `Entail [(s,TypeVar 0)] (c,TypeVar 0)`
+* will be in the set ie *)
+(* This should be equivalent to `entail` after turning all the super classes
+* and instance declarations to ie *)
 Inductive has_dict:
 [~lie:]
   p ∈ lie ⇒ has_dict ie lie p
 [~ie:]
-  it ∈ ie ∧ specialises_inst it (Instance cstrs p) ∧
-  (∀cstr. MEM cstr cstrs ⇒ has_dict ie lie cstr) ⇒ 
-    entail_type ie lie p
+  it ∈ ie ∧ specialises_inst it (Entail cstrs p) ∧
+  has_dicts ie lie cstrs ⇒
+    has_dict ie lie p
+[~dicts:]
+  (∀p. MEM p ps ⇒ has_dict ie lie p) ⇒
+    has_dicts ie lie ps
 End
 
-Definition has_dicts_def:
-  has_dicts ps = (∀p. MEM p ps ⇒ has_dict ie lie p)
+Inductive construct_dict:
+[~lie:]
+  FLOOKUP lie d = SOME p ⇒
+    construct_dict ie lie p (pure_cexp$Var _ d)
+[~ie:]
+  FLOOKUP ie d = SOME it ∧
+  specialises_inst it (Entail cstrs p) ∧
+  construct_dicts ie lie cstrs ds ⇒
+    construct_dict ie lie p (pure_cexp$App _ (pure_cexp$Var _ d) ds)
+[~dicts:]
+  (LIST_REL (construct_dict ie lie) ps ds) ⇒
+    construct_dicts ie lie ps ds
 End
 
+Theorem has_dict_EXISTS_construct_dict:
+  (∀p. has_dict (FRANGE ie) (FRANGE lie) p ⇒
+    ∃(d: 'a cexp) . construct_dict ie lie p d) ∧
+  ∀ps. has_dicts (FRANGE ie) (FRANGE lie) ps ⇒
+    ∃(ds: 'a cexp list). construct_dicts ie lie ps ds
+Proof
+  ho_match_mp_tac has_dict_ind >>
+  rw[]
+  >- (
+    irule_at (Pos hd) construct_dict_lie >>
+    metis_tac[finite_mapTheory.FRANGE_FLOOKUP]
+  )
+  >- (
+    irule_at (Pos hd) construct_dict_ie >>
+    metis_tac[finite_mapTheory.FRANGE_FLOOKUP]
+  ) >>
+  irule_at (Pos hd) construct_dict_dicts >>
+  pop_assum mp_tac >>
+  Induct_on `ps` >>
+  rw[] >>
+  pop_assum $ strip_assume_tac o SRULE[DISJ_IMP_THM,FORALL_AND_THM] >>
+  last_x_assum drule >>
+  metis_tac[]
+QED
+
+Theorem construct_dict_IMP_has_dict:
+  (∀p (d:'a cexp). construct_dict ie lie p d ⇒
+    has_dict (FRANGE ie) (FRANGE lie) p) ∧
+  (∀ps (ds:'a cexp list). construct_dicts ie lie ps ds ⇒
+    has_dicts (FRANGE ie) (FRANGE lie) ps)
+Proof
+  ho_match_mp_tac construct_dict_ind >>
+  rw[]
+  >- (
+    irule has_dict_lie >>
+    metis_tac[finite_mapTheory.FRANGE_FLOOKUP]
+  )
+  >- (
+    irule has_dict_ie >>
+    metis_tac[finite_mapTheory.FRANGE_FLOOKUP]
+  ) >>
+  irule has_dict_dicts >>
+  rw[] >>
+  gvs[LIST_REL_EVERY_ZIP,EVERY_MEM,MEM_EL,PULL_EXISTS] >>
+  first_x_assum drule >>
+  pairarg_tac >>
+  gvs[] >>
+  drule EL_ZIP >>
+  rw[] >>
+  first_x_assum drule >>
+  rw[] >>
+  first_x_assum irule
+QED
+
+Definition LIST_REL3_def:
+  LIST_REL3 R [] [] [] = T ∧
+  LIST_REL3 R (a::as) (b::bs) (c::cs) = (R a b c ∧ LIST_REL3 R as bs cs) ∧
+  LIST_REL3 R _ _ _ = F
+End
+
+Theorem LIST_REL3_EL:
+  ∀R as bs cs.
+  LIST_REL3 R as bs cs ⇔
+    (LENGTH bs = LENGTH as ∧ LENGTH cs = LENGTH as ∧
+     (∀n. n < LENGTH as ⇒ R (EL n as) (EL n bs) (EL n cs)))
+Proof
+  ho_match_mp_tac LIST_REL3_ind >>
+  reverse $ rw[LIST_REL3_def]
+  >- (strip_tac >> gvs[]) >>
+  rw[EQ_IMP_THM] >>
+  gvs[]
+  >- (
+    simp[Once $ oneline EL] >>
+    CASE_TAC >>
+    simp[]
+  )
+  >- (first_x_assum $ qspec_then `0` mp_tac >> simp[]) >>
+  first_x_assum $ qspec_then `SUC n` mp_tac >> fs[]
+QED
+
+Theorem LIST_REL3_strongind:
+  ∀R P.
+    P [] [] [] ∧
+    (∀a b c as bs cs.
+      R a b c ∧ LIST_REL3 R as bs cs ∧ P as bs cs ⇒
+        P (a::as) (b::bs) (c::cs)) ⇒
+    ∀as bs cs. LIST_REL3 R as bs cs ⇒ P as bs cs
+Proof
+  rpt gen_tac >>
+  strip_tac >>
+  `∀R' as bs cs. LIST_REL3 R' as bs cs ⇒ R' = R ⇒
+    (P as bs cs) ∧ LIST_REL3 R as bs cs`
+    suffices_by rw[] >>
+  ho_match_mp_tac LIST_REL3_ind >>
+  rw[LIST_REL3_def] >>
+  gvs[]
+QED
+
+Theorem LIST_REL3_induct:
+  ∀R P.
+    P [] [] [] ∧
+    (∀a b c as bs cs.
+      R a b c ∧ P as bs cs ⇒
+        P (a::as) (b::bs) (c::cs)) ⇒
+    ∀as bs cs. LIST_REL3 R as bs cs ⇒ P as bs cs
+Proof
+  rpt gen_tac >>
+  strip_tac >>
+  `∀R' as bs cs. LIST_REL3 R' as bs cs ⇒ R' = R ⇒ P as bs cs`
+    suffices_by rw[] >>
+  ho_match_mp_tac LIST_REL3_ind >>
+  rw[LIST_REL3_def] >>
+  gvs[]
+QED
+
+Theorem LIST_REL3_mono[mono]:
+  (∀x y z. R1 x y z ⇒ R2 x y z) ⇒
+    LIST_REL3 R1 l1 l2 l3 ⇒ LIST_REL3 R2 l1 l2 l3
+Proof
+  strip_tac >>
+  `∀R l1 l2 l3. LIST_REL3 R l1 l2 l3 ⇒ R = R1 ⇒ LIST_REL3 R2 l1 l2 l3`
+    suffices_by rw[] >>
+  ho_match_mp_tac LIST_REL3_ind >>
+  rw[LIST_REL3_def] >>
+  gvs[]
+QED
+
+(*
+  The main typing relation.
+  type_tcexp :
+      (ns: exndef # typedefs)     -- type definitions for exceptions and datatypes
+   -> (ie: entailment set)        -- instance environment
+   -> (lie: (class # type) set)   -- local instance environment
+   -> (db: Kind list)             -- deBruijn indices in scope
+                                  --   (kind of each index)
+   -> (st: type list)             -- store typing
+   -> (env: (string # (num # Predtype)) list)
+                                  -- term variables associated to type schemes
+   -> tcexp -> tcexp              -- expression, elaborated expression,
+   -> type                        -- and its type
+*)
+(* It does four things:
+* 1. checks the type of the expression
+* 2. removes the user's type annotatoin
+* 3. elaborates the class constraints for the variable
+* 4. elaborates the poly type in every let binding
+*)
 Inductive type_tcexp:
+(* remove the user type annotation after class constraint elaboration *)
+[~UserAnnot:]
+  type_tcexp ns ie lie db st env e e' t ⇒
+    type_tcexp ns ie lie db st env (UserAnnot t e) e' t
+
 [~Var:]
   (ALOOKUP env x = SOME s ∧
-   specialises_pred (SND ns) db s pt ⇒
-      pred_type_tcexp ns ce ie lie db st env (Var NONE x) pt)
+   specialises_pred (SND ns) db s (Pred ps t) ∧
+   has_dicts ie lie ps ⇒
+      type_tcexp ns ie lie db st env (Var _ x) (Var ps x) t)
 
-[~VarSOME:]
-  (ALOOKUP env x = SOME s ∧
-   specialises_pred (SND ns) db s pt ∧
-   pt = Pred ps ut ∧ has_dicts ie lie ps ⇒
-      type_tcexp ns ce ie lie db st env (Var (SOME ut) x) pt)
-
-(* instantiate pred_type_tcexp to type_tcexp *)
-[~Rel:]
-  pred_type_tcexp ns ce ie lie db st env e (Pred ps t) ∧
-  has_dicts ie lie ps ⇒
-    type_tcexp ns ce ie lie db st env e t
-
-(* adding context to type_tcexp for pred_type_tcexp *)
 [~Pred:]
-  type_tcexp ns ce ie (lie ∪ set ps) db st env e t ∧
-  pred_type_well_scoped (Pred ps t) ⇒
-  pred_type_tcexp ns ce ie lie db st env e (Pred ps t)
+  type_tcexp ns ie (lie ∪ set ps) db st env e e' t ⇒
+    pred_type_tcexp ns ie lie db st env e e' (Pred ps t)
 
 [~Tuple:]
-  (LIST_REL (type_tcexp ns ce ie lie db st env) es ts ∧
-  (pt = cons_types (Atom $ CompPrimTy $ Tuple (LENGTH es)) ts) ∧
-  user_annot_ok ut pt ⇒
-     type_tcexp ns ce ie lie db st env ((Prim ut (Cons «») es):tcexp) pt)
+  LIST_REL3 (type_tcexp ns ie lie db st env) es es' ts ∧
+  (t = cons_types (Atom $ CompPrimTy $ Tuple (LENGTH ts)) ts) ⇒
+     type_tcexp ns ie lie db st env (Prim (Cons «») es) (Prim (Cons «») es') t
 
 [~App:]
-  (type_tcexp ns ce ie lie db st env e (Functions arg_tys ret_ty) ∧
-   LIST_REL (type_tcexp ns ce ie lie db st env) es arg_tys ∧ arg_tys ≠ [] ∧
-   user_annot_ok ut ret_ty ⇒
-      type_tcexp ns ce ie lie db st env (App ut e es) ret_ty)
+  type_tcexp ns ie lie db st env e e' (Functions arg_tys ret_ty) ∧
+  es ≠ [] ∧
+  LIST_REL3 (type_tcexp ns ie lie db st env) es es' arg_tys ⇒
+    type_tcexp ns ie lie db st env (App e es) (App e' es') ret_ty
 
 [~Let:]
-  (type_tcexp ns (db + new) (MAP (tshift new) st) (tshift_env new env) e1 t1 ∧
-   type_tcexp ns db st ((x,new,t1)::env) e2 t2 ⇒
-      type_tcexp ns ce ie lie db st env (Let ut (x,pt) e1 e2) t2)
-End
+  LENGTH new = n ∧
+  pred_type_tcexp ns ie lie (new ++ db) (MAP (tshift $ LENGTH new) st)
+    (tshift_env_pred (LENGTH new) env) e1 e1' pt1 ∧
+  (* enforces all variables in the predicates to be well scoped:
+   * rejects `Read a, Show a => String -> String` *)
+  pred_type_well_scoped pt1 ∧
+  type_tcexp ns ie lie db st ((x,new,pt1)::env) e2 e2' t2 ⇒
+     type_tcexp ns ie lie db st env (Let (x,NONE) e1 e2)
+        (Let (x,SOME (n,pt)) e1' e2') t2
 
+(* The poly type of the let binding is annotated by the user *)
+[~LetSOME:]
+  type_tcexp ns ie lie db st env (Let (x,NONE) e1 e2)
+    (Let (x,SOME (n,pt)) e1' e2') t2 ⇒
+      type_tcexp ns ie lie db st env (Let (x,SONE (n,pt)) e1 e2)
+        (Let (x,SOME (n,pt)) e1' e2') t2
 
 [~Lam:]
-  (EVERY (type_ok (SND ns) db) arg_tys ∧
-   LENGTH arg_tys = LENGTH xs ∧ arg_tys ≠ [] ∧
+  EVERY (type_ok (SND ns) db) args_tys ∧
+  args_tys ≠ [] ∧
+  (* forcing the length of vs to be the same as arg_tys and
+  * handle user annotations in vs with args_tys *)
+  LIST_REL (λot t'.
+    case ot of
+    | NONE => T
+    | SOME t => t = t') (MAP SND vs) arg_tys ∧
+  type_tcexp ns ie lie db st
+    (REVERSE (ZIP (MAP FST vs, MAP (λat. ([],Pred [] at)) arg_tys)) ++ env)
+    e e' ret_ty ⇒
+      type_tcexp ns ie lie db st env (Lam vs e) (Lam vs e')
+        (Functions args_tys ret_ty)
 
-   type_tcexp ns ce ie lie db st (REVERSE (ZIP (xs, MAP ($, []) arg_tys)) ++ env) e ret_ty
-      ⇒ type_tcexp ns ce ie lie db st env (Lam ut xs e) (Functions arg_tys ret_ty))
+[~Cons:]
+  (LIST_REL3 (type_tcexp (exndef,typedefs) ie lie db st env) es es' carg_ts ∧
+   EVERY (type_ok typedefs db) tyargs ∧
+   type_cons typedefs db (cname,carg_ts) (tyid,tyargs) ⇒
+      type_tcexp (exndef,typedefs) ie lie db st env
+        (Prim (Cons cname) es) (Prim (Cons cname) es')
+        (tcons_to_type (INL tyid) tyargs))
+(*
+[~Letrec:]
+  (LIST_REL () fns fns')
+  (LIST_REL
+    (λ((fn,ot),body) (vars,scheme).
+      type_tcexp ns (vars ++ db) (MAP (tshift $ LENGTH vars) st)
+        (tshift_env_pred (LENGTH vars) $
+          REVERSE (ZIP (MAP (FST o FST) fns,schemes)) ++ env)
+        body scheme)
+    fns schemes ∧
+   EVERY (type_scheme_ok (SND ns) db) schemes ∧ fns ≠ [] ∧
+   type_tcexp ns ie lie db st
+     (REVERSE (ZIP (MAP FST fns, schemes)) ++ env) e e' t ⇒
+   type_tcexp ns ie lie db st env (Letrec fns e) (Letrec fns' e') t)
+*)
 End
 
+(*
+* Dictionary construction given that we have the elaborated expression.
+* tcexp_construct_dict:
+*     ns: mlstring set                    all constructors
+* ->  ie: (mlstring |-> (class # type))   instance environment
+* -> lie: (mlstring |-> entailment)       local instance environment
+* -> env: mlstring set                    term variables in scope
+* ->  ps: tcexp                           elaborated expression
+* ->  ds:'a cexp                          translated cexp expression
+*)
+
+(* we need to record the variables/constructors to avoid name collision *)
+Inductive tcexp_construct_dict:
+[~Var:]
+  construct_dicts ie lie ps ds ⇒
+    tcexp_construct_dict ns ie lie env (Var ps x)
+      (pure_cexp$App _ (pure_cexp$Var _ x) ds)
+
+[~Pred:]
+  (* enforce all variables in vs are fresh *)
+  set (MAP FST vs) ∩ (FDOM lie ∪ FDOM ie ∪ env ∪ ns) = ∅ ∧
+  tcexp_construct_dict ns ie (lie |++ vs) env e de ∧
+  ps = MAP SND vs ⇒
+    pred_tcexp_construct_dict ns ie lie env (Pred ps t) e (pure_cexp$Lam _ (MAP FST vs) de)
+
+[~Let:]
+  pred_tcexp_construct_dict ns ie lie env pt e1 de1 ∧
+  tcexp_construct_dict ns ie lie (x INSERT env) e2 de2 ⇒
+    tcexp_construct_dict ns ie lie env
+      (typeclass_tcexp$Let (x,SOME (new,pt)) e1 e2)
+      (pure_cexp$Let _ x de1 de2)
+
+[~Letrec:]
+  LIST_REL
+    (λ((x,ot),e) (y,de).
+      x = y ∧ ∃new pt. ot = SOME (new,pt) ∧
+      pred_tcexp_construct_dict ns ie lie
+        (env ∪ set (MAP (FST o FST) fns)) pt e de)
+    fns dfns ∧
+  tcexp_construct_dict ns ie lie (env ∪ set (MAP (FST o FST) fns)) e2 de2 ∧
+  fns ≠ [] ⇒
+    tcexp_construct_dict ns ie lie env
+      (typeclass_tcexp$Letrec fns e) (pure_cexp$Letrec _ dfns de)
+
+[~Prim:]
+  LIST_REL (tcexp_construct_dict ns ie lie env) es des ⇒
+    tcexp_construct_dict ns ie lie env (Prim c es) (Prim _ c des)
+
+[~Lam:]
+  tcexp_construct_dict ns ie lie
+    (set (MAP FST xs) ∪ env) e de ⇒
+      type_tcexp ns ie lie env (Lam xs e) (Lam _ (MAP FST xs) de)
+
+[~App:]
+  tcexp_construct_dict ns ie lie env e1 de1 ∧
+  LIST_REL (tcexp_construct_dict ns ie lie env) es des ⇒
+    tcexp_construct_dict ns ie lie env (App e1 es) (App _ de1 des)
+
+(* TODO
+[~NestedCase:]
+  tcexp_construct_dict ns ie lie env (NestedCase e v p e1 pes)
+    (NestedCase e' v p e1' pes')
+*)
+End
+
+(*
 [~Ret:]
   (type_tcexp ns db st env e t ∧ user_annot_ok ut pt ⇒
       type_tcexp ns db st env (Prim ut (Cons «Ret») [e]) (M t))
-End
 
 [~Bind:]
   (type_tcexp ns db st env e1 (M t1) ∧
